Pull the program module out of the signature module

theories/Base.v
@@ -28,16 +28,18 @@
 
 From Coq Require Export
      Numbers.BinNums.
+From Coq Require Import
+     Program.Tactics.
 From Katamaran Require Export
      Context
      Environment
      Prelude
+     Syntax.BinOps
      Syntax.Registers
      Syntax.TypeDecl
      Syntax.Variables
      Tactics.
 From Katamaran Require Import
-     Syntax.BinOps
      Syntax.Expressions
      Syntax.Patterns
      Syntax.Terms
@@ -56,6 +58,138 @@ Module Type BaseMixin (Import TY : Types).
   Notation LCtx := (NCtx LVar Ty).
   Notation Valuation Σ := (@Env (Binding LVar Ty) (fun xt : Binding LVar Ty => Val (@type LVar Ty xt)) Σ).
   Notation CStore := (@NamedEnv PVar Ty Val).
+
+  Section PatternMatching.
+    Context {N : Set}.
+
+    Definition pattern_match_env_reverse {Σ : LCtx} {σ : Ty} {Δ : NCtx N Ty} (p : Pattern Δ σ) :
+      NamedEnv (Term Σ) Δ -> Term Σ σ :=
+      match p with
+      | pat_var x    => fun Ex => match env.snocView Ex with env.isSnoc _ t => t end
+      | pat_unit     => fun _ => term_val ty.unit tt
+      | pat_pair x y => fun Exy => match env.snocView Exy with
+                                     env.isSnoc Ex ty =>
+                                     match env.snocView Ex with
+                                       env.isSnoc _ tx => term_binop bop.pair tx ty
+                                     end
+                                   end
+      | pat_tuple p  => fun EΔ => term_tuple (tuple_pattern_match_env_reverse p EΔ)
+      | pat_record p => fun EΔ => term_record _ (record_pattern_match_env_reverse p EΔ)
+      end.
+
+    Lemma inst_tuple_pattern_match {Σ : LCtx} {σs : Ctx Ty} {Δ : NCtx N Ty}
+      (ι : Valuation Σ) (p : TuplePat σs Δ) (ts : Env (Term Σ) σs) :
+      inst (tuple_pattern_match_env p ts) ι =
+      tuple_pattern_match_env p (inst (T := fun Σ => Env (Term Σ) σs) ts ι).
+    Proof.
+      unfold inst at 1; cbn.
+      induction p; cbn.
+      - reflexivity.
+      - destruct (env.snocView ts); cbn.
+        f_equal. apply IHp.
+    Qed.
+
+    Lemma inst_tuple_pattern_match_reverse {Σ : LCtx} {σs : Ctx Ty} {Δ : NCtx N Ty}
+      (ι : Valuation Σ) (p : TuplePat σs Δ) (ts : NamedEnv (Term Σ) Δ) :
+      inst (tuple_pattern_match_env_reverse p ts) ι =
+      tuple_pattern_match_env_reverse p (inst (T := fun Σ => NamedEnv (Term Σ) Δ) ts ι).
+    Proof.
+      unfold inst at 1; cbn.
+      induction p; cbn.
+      - reflexivity.
+      - destruct (env.snocView ts); cbn.
+        f_equal. apply IHp.
+    Qed.
+
+    Lemma inst_record_pattern_match {Δ__R : NCtx recordf Ty} {Σ : LCtx} {Δ : NCtx N Ty}
+      (ι : Valuation Σ) (p : RecordPat Δ__R Δ) (ts : NamedEnv (Term Σ) Δ__R) :
+      inst (T := fun Σ => NamedEnv (Term Σ) Δ) (record_pattern_match_env p ts) ι =
+      record_pattern_match_env p (inst ts ι).
+    Proof.
+      unfold inst at 1; cbn.
+      induction p; cbn.
+      - reflexivity.
+      - destruct (env.snocView ts); cbn.
+        f_equal. apply IHp.
+    Qed.
+
+    Lemma inst_record_pattern_match_reverse {Δ__R : NCtx recordf Ty} {Σ : LCtx} {Δ : NCtx N Ty}
+      (ι : Valuation Σ) (p : RecordPat Δ__R Δ) (ts : NamedEnv (Term Σ) Δ) :
+      inst (record_pattern_match_env_reverse p ts) ι =
+      record_pattern_match_env_reverse p (inst (T := fun Σ => NamedEnv (Term Σ) Δ) ts ι).
+    Proof.
+      unfold inst at 1; cbn.
+      induction p; cbn.
+      - reflexivity.
+      - destruct (env.snocView ts); cbn.
+        f_equal. apply IHp.
+    Qed.
+
+    Lemma inst_pattern_match_env_reverse {Σ : LCtx} {σ : Ty} {Δ : NCtx N Ty}
+          (ι : Valuation Σ) (p : Pattern Δ σ) (ts : NamedEnv (Term Σ) Δ) :
+      inst (Inst := inst_term) (pattern_match_env_reverse p ts) ι =
+      pattern_match_env_val_reverse p (inst (T := fun Σ => NamedEnv (Term Σ) Δ) ts ι).
+    Proof.
+      induction p.
+      - now destruct (env.snocView ts).
+      - reflexivity.
+      - destruct (env.snocView ts).
+        now destruct (env.snocView E); cbn.
+      - cbn - [Val].
+        now rewrite inst_term_tuple, inst_tuple_pattern_match_reverse.
+      - cbn.
+        f_equal.
+        apply inst_record_pattern_match_reverse.
+    Qed.
+
+  End PatternMatching.
+
+  Import env.notations.
+
+  Definition seval_exp {Γ Σ} (δ : SStore Γ Σ) :
+    forall {σ} (e : Exp Γ σ), Term Σ σ :=
+    fix seval_exp {σ} (e : Exp Γ σ) : Term Σ σ :=
+      match e with
+      | exp_var ς                => δ.[??ς]
+      | exp_val σ v              => term_val σ v
+      | exp_binop op e1 e2       => term_binop op (seval_exp e1) (seval_exp e2)
+      | exp_neg e                => term_neg (seval_exp e)
+      | exp_not e                => term_not (seval_exp e)
+      | exp_inl e                => term_inl (seval_exp e)
+      | exp_inr e                => term_inr (seval_exp e)
+      | exp_list es              => term_list (List.map seval_exp es)
+      | exp_bvec es              => term_bvec (Vector.map seval_exp es)
+      | exp_tuple es             => term_tuple (env.map (@seval_exp) es)
+      | exp_union E K e          => term_union E K (seval_exp e)
+      | exp_record R es          => term_record R (env.map (fun _ => seval_exp) es)
+      end%exp.
+
+  Lemma eval_exp_inst {Γ Σ τ} (ι : Valuation Σ) (δΓΣ : SStore Γ Σ) (e : Exp Γ τ) :
+    eval e (inst δΓΣ ι) = inst (seval_exp δΓΣ e) ι.
+  Proof.
+    induction e; cbn; repeat f_equal; auto.
+    { unfold inst, inst_store, inst_env at 1; cbn.
+      now rewrite env.lookup_map.
+    }
+    2: {
+      induction es as [|eb n es IHes]; cbn in *.
+      { reflexivity. }
+      { destruct X as [-> Heqs].
+        change (inst_term ?ι ?t) with (inst ι t).
+        destruct (inst (seval_exp δΓΣ eb) ι);
+          cbn; f_equal; auto.
+      }
+    }
+    all: induction es; cbn in *; destruct_conjs; f_equal; auto.
+  Qed.
+
+  Lemma subst_seval {Γ τ Σ Σ'} (e : Exp Γ τ) (ζ : Sub Σ Σ') (δ : SStore Γ Σ) :
+    subst (T := fun Σ => Term Σ _) (seval_exp δ e) ζ = seval_exp (subst δ ζ) e.
+  Proof.
+    induction e; cbn; f_equal; auto.
+    { now rewrite (subst_lookup xInΓ). }
+    all: induction es; cbn in *; destruct_conjs; f_equal; auto.
+  Qed.
 
   (* Preciseness for spatial predicates *)
   Record Precise {P : Set} (F : P -> Ctx Ty) (p : P) : Set :=
