theories/Specification.v
@@ -35,186 +35,36 @@ From Coq Require Import
      String.
 
 From Katamaran Require Export
-     Context
-     Environment
      Base
      Program
-     Syntax.Assertions
-     Syntax.BinOps
-     Syntax.Chunks
-     Syntax.Formulas
-     Syntax.Predicates
-     Syntax.ContractDecl
-     Symbolic.Propositions.
-From Katamaran Require Import
-     Symbolic.Worlds.
+     Signature.
 
 Import ctx.notations.
 Import env.notations.
 
-Local Set Implicit Arguments.
-Local Unset Transparent Obligations.
-Obligation Tactic := idtac.
+Module Type SpecificationMixin (B : Base) (Import P : Program B) (Import SIG : Signature B).
 
-Module Type ProgSpecMixinOn (Import B : Base) (Import P : Program B).
+  Definition SepContractEnv : Type :=
+    forall Δ τ (f : 𝑭 Δ τ), option (SepContract Δ τ).
+  Definition SepContractEnvEx : Type :=
+    forall Δ τ (f : 𝑭𝑿 Δ τ), SepContract Δ τ.
+  Definition LemmaEnv : Type :=
+    forall Δ (l : 𝑳 Δ), Lemma Δ.
 
-  Section PatternMatching.
+End SpecificationMixin.
 
-    Context {N : Set}.
+Module Type SpecificationKit (B : Base) (P : Program B)
+  (Import SIG : Signature B) (Import SM : SpecificationMixin B P SIG).
 
-    Definition pattern_match_env_reverse {Σ : LCtx} {σ : Ty} {Δ : NCtx N Ty} (p : Pattern Δ σ) :
-      NamedEnv (Term Σ) Δ -> Term Σ σ :=
-      match p with
-      | pat_var x    => fun Ex => match env.snocView Ex with env.isSnoc _ t => t end
-      | pat_unit     => fun _ => term_val ty.unit tt
-      | pat_pair x y => fun Exy => match env.snocView Exy with
-                                     env.isSnoc Ex ty =>
-                                     match env.snocView Ex with
-                                       env.isSnoc _ tx => term_binop bop.pair tx ty
-                                     end
-                                   end
-      | pat_tuple p  => fun EΔ => term_tuple (tuple_pattern_match_env_reverse p EΔ)
-      | pat_record p => fun EΔ => term_record _ (record_pattern_match_env_reverse p EΔ)
-      end.
+  Local Set Implicit Arguments.
 
-    Lemma inst_tuple_pattern_match {Σ : LCtx} {σs : Ctx Ty} {Δ : NCtx N Ty}
-      (ι : Valuation Σ) (p : TuplePat σs Δ) (ts : Env (Term Σ) σs) :
-      inst (tuple_pattern_match_env p ts) ι =
-      tuple_pattern_match_env p (inst (T := fun Σ => Env (Term Σ) σs) ts ι).
-    Proof.
-      unfold inst at 1; cbn.
-      induction p; cbn.
-      - reflexivity.
-      - destruct (env.snocView ts); cbn.
-        f_equal. apply IHp.
-    Qed.
+  Parameter CEnv   : SepContractEnv.
+  Parameter CEnvEx : SepContractEnvEx.
+  Parameter LEnv   : LemmaEnv.
 
-    Lemma inst_tuple_pattern_match_reverse {Σ : LCtx} {σs : Ctx Ty} {Δ : NCtx N Ty}
-      (ι : Valuation Σ) (p : TuplePat σs Δ) (ts : NamedEnv (Term Σ) Δ) :
-      inst (tuple_pattern_match_env_reverse p ts) ι =
-      tuple_pattern_match_env_reverse p (inst (T := fun Σ => NamedEnv (Term Σ) Δ) ts ι).
-    Proof.
-      unfold inst at 1; cbn.
-      induction p; cbn.
-      - reflexivity.
-      - destruct (env.snocView ts); cbn.
-        f_equal. apply IHp.
-    Qed.
+End SpecificationKit.
 
-    Lemma inst_record_pattern_match {Δ__R : NCtx recordf Ty} {Σ : LCtx} {Δ : NCtx N Ty}
-      (ι : Valuation Σ) (p : RecordPat Δ__R Δ) (ts : NamedEnv (Term Σ) Δ__R) :
-      inst (T := fun Σ => NamedEnv (Term Σ) Δ) (record_pattern_match_env p ts) ι =
-      record_pattern_match_env p (inst ts ι).
-    Proof.
-      unfold inst at 1; cbn.
-      induction p; cbn.
-      - reflexivity.
-      - destruct (env.snocView ts); cbn.
-        f_equal. apply IHp.
-    Qed.
-
-    Lemma inst_record_pattern_match_reverse {Δ__R : NCtx recordf Ty} {Σ : LCtx} {Δ : NCtx N Ty}
-      (ι : Valuation Σ) (p : RecordPat Δ__R Δ) (ts : NamedEnv (Term Σ) Δ) :
-      inst (record_pattern_match_env_reverse p ts) ι =
-      record_pattern_match_env_reverse p (inst (T := fun Σ => NamedEnv (Term Σ) Δ) ts ι).
-    Proof.
-      unfold inst at 1; cbn.
-      induction p; cbn.
-      - reflexivity.
-      - destruct (env.snocView ts); cbn.
-        f_equal. apply IHp.
-    Qed.
-
-    Lemma inst_pattern_match_env_reverse {Σ : LCtx} {σ : Ty} {Δ : NCtx N Ty}
-          (ι : Valuation Σ) (p : Pattern Δ σ) (ts : NamedEnv (Term Σ) Δ) :
-      inst (Inst := inst_term) (pattern_match_env_reverse p ts) ι =
-      pattern_match_env_val_reverse p (inst (T := fun Σ => NamedEnv (Term Σ) Δ) ts ι).
-    Proof.
-      induction p.
-      - now destruct (env.snocView ts).
-      - reflexivity.
-      - destruct (env.snocView ts).
-        now destruct (env.snocView E); cbn.
-      - cbn - [Val].
-        now rewrite inst_term_tuple, inst_tuple_pattern_match_reverse.
-      - cbn.
-        f_equal.
-        apply inst_record_pattern_match_reverse.
-    Qed.
-
-  End PatternMatching.
-
-  Definition seval_exp {Γ Σ} (δ : SStore Γ Σ) :
-    forall {σ} (e : Exp Γ σ), Term Σ σ :=
-    fix seval_exp {σ} (e : Exp Γ σ) : Term Σ σ :=
-      match e with
-      | exp_var ς                => δ.[??ς]
-      | exp_val σ v              => term_val σ v
-      | exp_binop op e1 e2       => term_binop op (seval_exp e1) (seval_exp e2)
-      | exp_neg e                => term_neg (seval_exp e)
-      | exp_not e                => term_not (seval_exp e)
-      | exp_inl e                => term_inl (seval_exp e)
-      | exp_inr e                => term_inr (seval_exp e)
-      | exp_list es              => term_list (List.map seval_exp es)
-      | exp_bvec es              => term_bvec (Vector.map seval_exp es)
-      | exp_tuple es             => term_tuple (env.map (@seval_exp) es)
-      | exp_union E K e          => term_union E K (seval_exp e)
-      | exp_record R es          => term_record R (env.map (fun _ => seval_exp) es)
-      end%exp.
-
-  Lemma eval_exp_inst {Γ Σ τ} (ι : Valuation Σ) (δΓΣ : SStore Γ Σ) (e : Exp Γ τ) :
-    eval e (inst δΓΣ ι) = inst (seval_exp δΓΣ e) ι.
-  Proof.
-    induction e; cbn; repeat f_equal; auto.
-    { unfold inst, inst_store, inst_env at 1; cbn.
-      now rewrite env.lookup_map.
-    }
-    2: {
-      induction es as [|eb n es IHes]; cbn in *.
-      { reflexivity. }
-      { destruct X as [-> Heqs].
-        change (inst_term ?ι ?t) with (inst ι t).
-        destruct (inst (seval_exp δΓΣ eb) ι);
-          cbn; f_equal; auto.
-      }
-    }
-    all: induction es; cbn in *; destruct_conjs; f_equal; auto.
-  Qed.
-
-  Lemma subst_seval {Γ τ Σ Σ'} (e : Exp Γ τ) (ζ : Sub Σ Σ') (δ : SStore Γ Σ) :
-    subst (T := fun Σ => Term Σ _) (seval_exp δ e) ζ = seval_exp (subst δ ζ) e.
-  Proof.
-    induction e; cbn; f_equal; auto.
-    { now rewrite (subst_lookup xInΓ). }
-    all: induction es; cbn in *; destruct_conjs; f_equal; auto.
-  Qed.
-
-End ProgSpecMixinOn.
-
-Module Type SpecificationMixin (B : Base) (P : Program B) (CD : ContractDecl B P) :=
-  ProgSpecMixinOn B P <+ WorldsOn B CD CD <+ SymPropOn B CD CD CD.
-
-Module Type ProgramLogicSignature (B : Base).
-  Declare Module Export PROG : Program B.
-  Include PredicateKit B.
-  Include ContractDeclMixin B PROG.
-  Include SpecificationMixin B PROG.
-End ProgramLogicSignature.
-
-Module Type Specification (B : Base) (Import SIG : ProgramLogicSignature B).
-  Include ContractDefKit B PROG SIG.
+Module Type Specification (B : Base) (P : Program B) (SIG : Signature B).
+  Include SpecificationMixin B P SIG.
+  Include SpecificationKit B P SIG.
 End Specification.
-
-Module Type SolverKit (B : Base) (Import SIG : ProgramLogicSignature B).
-
-  Parameter solver      : Solver.
-  Parameter solver_spec : SolverSpec solver.
-
-End SolverKit.
-
-Module DefaultSolverKit (B : Base) (Import SIG : ProgramLogicSignature B) <: SolverKit B SIG.
-
-  Definition solver : Solver := solver_null.
-  Definition solver_spec : SolverSpec solver := solver_null_spec.
-
-End DefaultSolverKit.
